verif/trie/common.v
@@ -1,5 +1,5 @@
 (** * common.v : Common definitions *)
-Require Import VST.floyd.functional_base.
+Require Import VST.floyd.proofauto.
 Definition string := list byte.
 Instance EqDec_string: EqDec string := list_eq_dec Byte.eq_dec.
 
@@ -8,3 +8,26 @@ Module Type VALUE_TYPE.
   Parameter default: type.
   Parameter inhabitant_value: Inhabitant type.
 End VALUE_TYPE.
+
+Ltac elim_cast_pointer' term t :=
+  match t with
+  | force_val (sem_cast_pointer ?t') => elim_cast_pointer' term t'
+  | _ =>
+    let H := fresh "H" in
+    first [
+        apply (assert_later_PROP (is_pointer_or_null t))
+      | apply (assert_PROP (is_pointer_or_null t))
+      | apply (assert_PROP' (is_pointer_or_null t))];
+    [ now entailer!
+    | intro H ];
+    idtac term;
+    idtac t;
+    replace term with t by (destruct t; first [contradiction | reflexivity]);
+    clear H
+  end.
+
+Ltac elim_cast_pointer :=
+  match goal with
+  | |- context [force_val (sem_cast_pointer ?t)] =>
+    elim_cast_pointer' (force_val (sem_cast_pointer t)) t
+  end.
