verif/trie/util.v
@@ -484,7 +484,7 @@ Definition f_UTIL_GetNextKeySlice := {|
                                  tvoid cc_default))
           ((Evar ___stringlit_4 (tarray tschar 9)) ::
            (Evar ___stringlit_1 (tarray tschar 7)) ::
-           (Econst_int (Int.repr 106) tint) ::
+           (Econst_int (Int.repr 105) tint) ::
            (Evar ___func____1 (tarray tschar 21)) :: nil)))
       (Ssequence
         (Sifthenelse (Ebinop Ole (Etempvar _len tint)
@@ -499,7 +499,7 @@ Definition f_UTIL_GetNextKeySlice := {|
                                    cc_default))
             ((Evar ___stringlit_5 (tarray tschar 35)) ::
              (Evar ___stringlit_1 (tarray tschar 7)) ::
-             (Econst_int (Int.repr 107) tint) ::
+             (Econst_int (Int.repr 106) tint) ::
              (Evar ___func____1 (tarray tschar 21)) :: nil)))
         (Ssequence
           (Swhile
@@ -579,7 +579,7 @@ Definition f_UTIL_KeySliceToStr := {|
                                tvoid cc_default))
         ((Evar ___stringlit_4 (tarray tschar 9)) ::
          (Evar ___stringlit_1 (tarray tschar 7)) ::
-         (Econst_int (Int.repr 128) tint) ::
+         (Econst_int (Int.repr 127) tint) ::
          (Evar ___func____2 (tarray tschar 19)) :: nil)))
     (Ssequence
       (Sifthenelse (Ebinop Ole (Etempvar _len tint)
@@ -593,7 +593,7 @@ Definition f_UTIL_KeySliceToStr := {|
                                  tvoid cc_default))
           ((Evar ___stringlit_5 (tarray tschar 35)) ::
            (Evar ___stringlit_1 (tarray tschar 7)) ::
-           (Econst_int (Int.repr 129) tint) ::
+           (Econst_int (Int.repr 128) tint) ::
            (Evar ___func____2 (tarray tschar 19)) :: nil)))
       (Ssequence
         (Ssequence
